utils/Zeta.SeqIdx.fst
@@ -1,0 +1,43 @@
+module Zeta.SeqIdx
+
+let exists_elems_with_prop_comp (#a:_) (p: a -> bool) (s: seq a)
+  : b:bool {b <==> exists_elems_with_prop p s}
+  = admit()
+
+let exists_elems_with_prop_intro (#a:_) (p: a -> bool) (s: seq a) (i: seq_index s{p (index s i)})
+  : Lemma (ensures (exists_elems_with_prop p s))
+  = admit()
+
+let last_idx (#a:_) (p: a -> bool) (s: seq a {exists_elems_with_prop p s})
+  : i:seq_index s{p (index s i)}
+  = admit()
+
+let last_idx_snoc (#a:_) (p: a -> bool) (s: seq a {length s > 0})
+  : Lemma (ensures (let i = length s - 1 in
+                    let s' = prefix s i in
+                    p (index s i) /\ last_idx p s = i \/
+                    ~ (p (index s i))  /\
+                    (exists_elems_with_prop p s <==> exists_elems_with_prop p s') /\
+                    (exists_elems_with_prop p s' ==> last_idx p s = last_idx p s')))
+  = admit()
+
+let last_idx_correct (#a:_) (p: a -> bool)
+  (s: seq a{exists_elems_with_prop p s})
+  (i: seq_index s)
+  : Lemma (ensures ((i > last_idx p s ==> ~ (p (index s i))) /\
+                    (p (index s i) ==> i <= last_idx p s)))
+  = admit()
+
+let next_idx (#a:_) (p: a -> bool)
+  (s: seq a {exists_elems_with_prop p s})
+  (i: seq_index s{i < last_idx p s})
+  : j:seq_index s{p (index s j) /\ j > i /\ j <= (last_idx p s)}
+  = admit()
+
+let next_idx_correct (#a:_) (p: a -> bool)
+  (s: seq a {exists_elems_with_prop p s})
+  (i: seq_index s {i < last_idx p s})
+  : Lemma (ensures (let j = next_idx p s i in
+                    let s' = prefix s j in
+                    exists_elems_with_prop p s' ==> last_idx p s' <= i))
+  = admit()
